custom induction for equiv_val

coq/stlc3.v
@@ -155,6 +155,56 @@ with equiv_env : stack vl_stack -> venv -> venv_stack -> Prop :=
                       equiv_env lS (Def vl H1 (H2++H20) (length H20)) (H1s, (H2s, length H20)) 
 .
 
+Print Forall2_ind.
+Print equiv_val_ind.
+Print equiv_env_ind.
+
+
+Definition eqv_nested_ind := fun
+  (Pv : stack vl_stack -> vl -> vl_stack -> Prop)
+  (Pe : stack vl_stack -> venv -> venv_stack -> Prop)
+  (fconst : forall (b : bool) (st : stack vl_stack),
+       Pv st (vbool b) (vbool_stack b))
+  (fabs : forall (H1 H2 : list vl) (idx : nat) (lS : stack vl_stack)
+          (i : st_ptr) (t : tm) (n : class) (H : heap vl_stack)
+          (fr : list vl_stack),
+        get_stack_frame lS i = Some (fr, idx) ->
+        Pe lS (Def vl H1 H2 idx) (H, (fr, idx)) ->
+        Pv lS (vabs (Def vl H1 H2 idx) n t) (vabs_stack H i n t))
+  (fenv : forall (lS : stack vl_stack) (H1 : list vl) 
+         (H1s : list vl_stack) (H2 : list vl) (H2s : list vl_stack)
+         (H20 : list vl),
+       Forall2 (fun (v : vl) (vs : vl_stack) => Pv lS v vs) H1 H1s ->
+       Forall2 (fun (v : vl) (vs : vl_stack) => Pv lS v vs) H2 H2s ->
+       Pe lS (Def vl H1 (H2 ++ H20) (length H20)) (H1s, (H2s, length H20)))
+=>
+  fix F (s : stack vl_stack) (v : vl) (v0 : vl_stack) (e : equiv_val s v v0): Pv s v v0 :=
+match e in (equiv_val s0 v1 v2) return (Pv s0 v1 v2) with
+| equiv_const x x0 => fconst x x0
+| equiv_abs x x0 x1 x2 x3 x4 x5 x6 x7 x8 x9 =>
+  fabs x x0 x1 x2 x3 x4 x5 x6 x7 x8 (
+         match x9 in (equiv_env s0 v1 v2) return (Pe s0 v1 v2) with
+           | eqv_forall x x0 x1 x2 x3 x4 x5 x6 =>
+             fenv x x0 x1 x2 x3 x4
+                  ((fix G l l' (fa: Forall2 (fun v v' => equiv_val x v v') l l') := match fa in (Forall2 _ l1 l2) return Forall2 _ l1 l2 with
+                                | Forall2_nil => Forall2_nil _
+                                | Forall2_cons a b x1 x2 r x4 =>
+                                  Forall2_cons a b (F x a b r) (G x1 x2 x4)
+                              end) x0 x1 x5)
+                  ((fix G l l' (fa: Forall2 (fun v v' => equiv_val x v v') l l') := match fa in (Forall2 _ l1 l2) return Forall2 _ l1 l2 with
+                                | Forall2_nil => Forall2_nil _
+                                | Forall2_cons a b x1 x2 r x4 =>
+                                  Forall2_cons a b (F x a b r) (G x1 x2 x4)
+                              end) x2 x3 x6)
+         end)
+end.
+
+
+
+
+
+
+
 
 Inductive equiv_opt: stack vl_stack -> option (vl) -> option (vl_stack) -> Prop :=
 | e_stuck : forall lS, equiv_opt lS None None
@@ -285,7 +335,18 @@ Lemma stack_extend_val : forall lS v v' fr,
    equiv_val lS v v' ->
    equiv_val (fr::lS) v v'.
 Proof.
-   Admitted.
+  intros. 
+  eapply (eqv_nested_ind
+            (fun lS v v' => equiv_val (fr::lS) v v')
+            (fun lS v v' => equiv_env (fr::lS) v v')).
+
+  - intros. constructor.
+  - intros. econstructor. destruct i. simpl. eauto. simpl. eauto. simpl in H3.
+    assert (beq_nat n0 (length lS0) = false). admit. (* from index_max *)
+    rewrite H5. eauto. eauto.
+  - intros. constructor; eauto.
+  - eauto.
+Qed.
 
 Lemma stack_extend : forall lS env env' fr, 
    equiv_env lS env env' ->
